Deploying to gh-pages from @ xubaiw/reservoir-index@a16228cb061b234cab087f807984b0261e2869fa 🚀

git/siddhartha-gadgil/Polylean/Polylean/GroupRing.lean
@@ -1,3 +1,262 @@
+import Polylean.FreeModule
+
 /-
 Group ring given a group. The ring structures is constructed using the universal property of R-modules, with uniqueness used to show that it is a ring. This is only an additional structure, i.e., no need to wrap. 
 -/
+
+variable (R : Type) [Ring R] [DecidableEq R]
+
+variable (G: Type) [Group G] [DecidableEq G]
+
+
+def FormalSum.mulTerm (b: R)(h: G) : FormalSum R G → FormalSum R G 
+| [] => []
+| (a, g) :: tail => (a * b, g * h) :: (mulTerm b h tail)
+
+def FormalSum.mul(fst: FormalSum R G) : FormalSum R G → FormalSum R G
+| [] =>    []
+| (b, h) :: ys =>  
+  (FormalSum.mulTerm R G b h fst) ++ (mul fst ys)
+
+open FormalSum
+
+theorem mulTerm_zero (g x₀: G)(s: FormalSum R G):
+  coords (mulTerm R G 0 g s) x₀ = 0 := by
+  induction s with
+  | nil =>  
+    simp [mulTerm, coords]
+  | cons h t ih => 
+    simp [mulTerm, coords, monom_coords_at_zero]
+    assumption
+
+theorem mulTerm_add(b₁ b₂ : R)(h : G)(s: FormalSum R G):
+  coords (mulTerm R G (b₁ + b₂) h s) x₀ = coords (mulTerm R G b₁ h s) x₀ + coords (mulTerm R G b₂ h s) x₀ := by
+  induction s with
+  | nil => 
+  simp [mulTerm, coords]
+  | cons head tail ih => 
+    let (a, g) := head
+    simp [mulTerm, coords]
+    rw [left_distrib]
+    rw [monom_coords_hom]
+    rw [ih]
+    conv =>
+      lhs
+      rw [add_assoc]
+      congr
+      skip
+      rw [← add_assoc]
+      congr
+      rw [add_comm]    
+    conv =>
+      rhs
+      rw [add_assoc]
+    conv =>
+      rhs 
+      congr
+      skip 
+      rw [← add_assoc]
+
+theorem mul_zero_cons (s t : FormalSum R G)(g: G): 
+    mul R G s ((0, h) :: t) ≈  mul R G s t := by
+    induction s
+    case nil =>
+      simp [mul, mulTerm]
+      apply eqlCoords.refl
+    case cons head tail ih =>
+      simp [mul, mulTerm]
+      apply funext ; intro x₀
+      simp [coords]
+      rw [monom_coords_at_zero]
+      rw [zero_add]
+      rw [← append_coords]
+      simp [coords, mul]
+      let l := mulTerm_zero R G h x₀ tail
+      rw [l]
+      simp [zero_add]
+
+  
+def mulAux : FormalSum R G → FreeModule R G → FreeModule R G := by
+  intro s
+  let f  := fun t => ⟦ FormalSum.mul R G s t ⟧ 
+  apply  Quotient.lift f
+  apply func_eql_of_move_equiv
+  intro t t' rel
+  simp 
+  induction rel with
+  | zeroCoeff tail g a hyp =>
+    rw [hyp]
+    apply Quotient.sound
+    simp [mul]
+    apply funext
+    intro x₀
+    rw [← append_coords]
+    let l := mulTerm_zero R G g x₀ s
+    rw [l]
+    simp [zero_add]
+  | addCoeffs a b x tail =>
+    apply Quotient.sound
+    apply funext; intro x₀
+    simp [mul]
+    repeat (rw [← append_coords])
+    simp
+    simp [mulTerm_add, add_assoc]    
+  | cons a x s₁ s₂ r step =>
+    apply Quotient.sound
+    apply funext ; intro x₀
+    simp [mul]
+    rw [← append_coords]
+    rw [← append_coords]
+    simp 
+    let l := Quotient.exact step
+    let l := congrFun l x₀
+    rw [l]
+  | swap a₁ a₂ x₁ x₂ tail =>
+    apply Quotient.sound
+    apply funext ; intro x₀
+    simp [mul, ← append_coords]
+    rw [← add_assoc]
+    rw [← add_assoc]
+    simp
+    let lc := 
+      add_comm 
+        (coords (mulTerm R G a₁ x₁ s) x₀)
+        (coords (mulTerm R G a₂ x₂ s) x₀)
+    rw [lc] 
+
+open ElementaryMove
+theorem mulTerm_invariant (b : R)(h x₀ : G)(s₁ s₂ : FormalSum R G)
+    (rel : ElementaryMove R G s₁ s₂) : 
+      coords (mulTerm R G b h s₁) x₀ = 
+      coords (mulTerm R G b h s₂) x₀ := by
+      induction rel with
+      | zeroCoeff tail g a hyp => 
+        rw [hyp]
+        simp [mulTerm, coords,monom_coords_at_zero]
+      | addCoeffs a₁ a₂ x tail => 
+        simp [mulTerm, coords, right_distrib, monom_coords_hom, add_assoc]
+        
+      | cons a x t₁ t₂ r step => 
+        simp [mulTerm, coords, step]
+      | swap a₁ a₂ x₁ x₂ tail => 
+        simp [mulTerm, coords]
+        conv =>
+          lhs
+          rw [← add_assoc]
+          arg 1
+          rw [add_comm]
+        rw [← add_assoc]      
+
+
+theorem first_arg_invariant (s₁ s₂ t : FormalSum R G) 
+  (rel : ElementaryMove R G s₁ s₂) :
+    FormalSum.mul R G s₁ t ≈  FormalSum.mul R G s₂ t := by 
+    cases t
+    case nil => 
+      simp [mul]
+      rfl
+    case cons head' tail' =>
+      let (b, h) := head'
+      induction rel with
+      | zeroCoeff tail g a hyp => 
+        rw [hyp]
+        simp [mul, mulTerm]
+        apply funext; intro x₀
+        rw [← append_coords]
+        simp
+        simp [coords, monom_coords_at_zero]
+        rw [← append_coords]
+        simp  
+        let rel' : ElementaryMove R G ((0, g) :: tail)  tail := by 
+          apply ElementaryMove.zeroCoeff
+          rfl
+        let prev  := first_arg_invariant  _ _ tail' rel' 
+        let pl := congrFun prev x₀
+        rw [pl]  
+      | addCoeffs a₁ a₂ x tail => 
+        simp [mul]
+        apply funext; intro x₀
+        rw [← append_coords]
+        rw [← append_coords]
+        simp [coords]
+        rw [right_distrib]
+        simp [monom_coords_hom]
+        let rel' : ElementaryMove R G 
+          ((a₁, x) :: (a₂, x) :: tail)
+            ((a₁ + a₂, x) :: tail) := by 
+            apply ElementaryMove.addCoeffs
+        let prev  := first_arg_invariant  _ _ tail' rel' 
+        let pl := congrFun prev x₀
+        rw [pl]
+        simp [add_assoc] 
+      | cons a x s₁ s₂ r step => 
+        simp [mul]
+        apply funext; intro x₀
+        rw [← append_coords]
+        rw [← append_coords]
+        simp [coords]
+        let rel' : ElementaryMove R G 
+          ((a, x) :: s₁)
+            ((a, x) :: s₂) := by 
+            apply ElementaryMove.cons
+            assumption 
+        let prev  := first_arg_invariant  _ _ tail' rel' 
+        let pl := congrFun prev x₀
+        rw [pl]
+        let ps := mulTerm_invariant R G b h x₀ s₁ s₂ r
+        rw [ps]       
+      | swap a₁ a₂ x₁ x₂ tail => 
+        simp [mul]
+        apply funext; intro x₀
+        rw [← append_coords]
+        rw [← append_coords]
+        simp
+        rw [mulTerm]
+        rw [mulTerm]
+        rw [coords]
+        rw [coords]
+        rw [mulTerm]
+        rw [mulTerm]
+        rw [coords]
+        rw [coords]
+        simp
+        let rel' : ElementaryMove R G 
+          ((a₁, x₁) :: (a₂, x₂) :: tail)
+            ((a₂, x₂) :: (a₁, x₁) :: tail) := by 
+            apply ElementaryMove.swap
+        let prev  := first_arg_invariant  _ _ tail' rel' 
+        let pl := congrFun prev x₀
+        rw [pl]
+        simp 
+        rw [← add_assoc]
+        rw [← add_assoc]
+        simp
+        conv =>
+          lhs 
+          congr
+          congr
+          rw [add_comm]    
+        
+
+
+
+def FreeModule.mul : FreeModule R G → FreeModule R G → FreeModule R G := by
+  let f  := fun (s : FormalSum R G) => 
+    fun  (t : FreeModule R G) => mulAux R G s t 
+  apply  Quotient.lift f
+  apply func_eql_of_move_equiv  
+  intro s₁ s₂ rel
+  simp 
+  apply funext
+  apply Quotient.ind 
+  intro t
+  let lhs : mulAux R G s₁ (Quotient.mk (formalSumSetoid R G) t) = 
+    ⟦FormalSum.mul R G s₁ t⟧ := by rfl
+  let rhs : mulAux R G s₂ (Quotient.mk (formalSumSetoid R G) t) = 
+    ⟦FormalSum.mul R G s₂ t⟧ := by rfl
+  rw [lhs, rhs]
+  simp
+  apply Quotient.sound
+  apply first_arg_invariant
+  exact rel
+  
